use specialized bignum for ecdsa-k256

code/k256/Hacl.Impl.K256.Verify.fst
@@ -8,10 +8,7 @@ open Lib.IntTypes
 open Lib.Buffer
 
 module ST = FStar.HyperStack.ST
-module LSeq = Lib.Sequence
 module BSeq = Lib.ByteSequence
-
-module BD = Hacl.Bignum.Definitions
 
 module QI = Hacl.Impl.K256.Qinv
 
@@ -23,6 +20,8 @@ open Hacl.K256.Scalar
 open Hacl.Impl.K256.Point
 open Hacl.Impl.K256.PointMul
 
+module BI = Hacl.Spec.K256.Field52
+module BL = Hacl.Spec.K256.Field52.Lemmas
 
 #set-options "--z3rlimit 50 --fuel 0 --ifuel 0"
 
@@ -36,6 +35,7 @@ val is_public_key_valid (pk_x pk_y:lbytes32) (fpk_x fpk_y:felem) : Stack bool
     disjoint fpk_x fpk_y /\ disjoint fpk_x pk_x /\ disjoint fpk_x pk_y /\
     disjoint fpk_y pk_y /\ disjoint fpk_y pk_x)
   (ensures  fun h0 b h1 -> modifies (loc fpk_x |+| loc fpk_y) h0 h1 /\
+    (b ==> inv_fully_reduced h1 fpk_x /\ inv_fully_reduced h1 fpk_y) /\
     (as_nat h1 fpk_x, as_nat h1 fpk_y, b) ==
       S.is_public_key_valid (as_seq h0 pk_x) (as_seq h0 pk_y))
 
@@ -61,8 +61,8 @@ val ecdsa_verify_qelem (res p:point) (z r s:qelem) : Stack unit
    (let sinv = S.qinv (qas_nat h0 s) in
     let u1 = S.qmul (qas_nat h0 z) sinv in
     let u2 = S.qmul (qas_nat h0 r) sinv in
-    S.to_aff_point (point_as_nat3_proj h1 res) ==
-    S.to_aff_point (S.point_mul_double_g u1 u2 (point_as_nat3_proj h0 p))))
+    S.to_aff_point (point_eval h1 res) ==
+    S.to_aff_point (S.point_mul_double_g u1 u2 (point_eval h0 p))))
 
 let ecdsa_verify_qelem res p z r s =
   push_frame ();
@@ -80,15 +80,21 @@ let ecdsa_verify_qelem res p z r s =
 val fmul_eq_vartime (r z x: felem) : Stack bool
   (requires fun h ->
     live h r /\ live h z /\ live h x /\ eq_or_disjoint r z /\
-    fe_lt_prime h r /\ fe_lt_prime h z /\ fe_lt_prime h x)
+    felem_fits5 (as_felem5 h r) (2,2,2,2,2) /\ as_nat h r < S.prime /\
+    inv_lazy_reduced2 h z /\ inv_fully_reduced h x)
   (ensures  fun h0 b h1 -> modifies0 h0 h1 /\
-    b == (S.fmul (as_nat h0 r) (as_nat h0 z) = as_nat h0 x))
+    b == (S.fmul (as_nat h0 r) (feval h0 z) = as_nat h0 x))
 
 [@CInline]
 let fmul_eq_vartime r z x =
   push_frame ();
   let tmp = create_felem () in
   fmul tmp r z;
+  let h1 = ST.get () in
+  fnormalize tmp tmp;
+  let h2 = ST.get () in
+  BL.normalize5_lemma (1,1,1,1,2) (as_felem5 h1 tmp);
+  assert (inv_fully_reduced h2 tmp);
   let b = is_felem_eq_vartime tmp x in
   pop_frame ();
   b
@@ -99,35 +105,56 @@ val ecdsa_verify_avoid_finv: p:point -> r:qelem -> Stack bool
   (requires fun h ->
     live h p /\ live h r /\ disjoint p r /\
     point_inv h p /\ qe_lt_q h r /\ 0 < qas_nat h r /\
-    not (S.is_proj_point_at_inf (point_as_nat3_proj h p)))
+    not (S.is_proj_point_at_inf (point_eval h p)))
   (ensures  fun h0 b h1 -> modifies0 h0 h1 /\
-    (let (_X, _Y, _Z) = point_as_nat3_proj h0 p in
+    (let (_X, _Y, _Z) = point_eval h0 p in
      b <==> (S.fmul _X (S.finv _Z) % S.q = qas_nat h0 r)))
 
 let ecdsa_verify_avoid_finv p r =
-  push_frame ();
   let h0 = ST.get () in
+  let x, y, z = getx p, gety p, getz p in
+
+  push_frame ();
   let r_bytes = create 32ul (u8 0) in
   let r_fe = create_felem () in
-  let tmp = create_felem () in
+  let tmp_q = create_felem () in
+  let tmp_x = create_felem () in
 
   store_qelem r_bytes r;
   load_felem r_fe r_bytes;
+  let h1 = ST.get () in
+  //assert (inv_fully_reduced h1 r_fe);
+  //assert (as_nat h1 r_fe == qas_nat h1 r);
 
-  let x, y, z = getx p, gety p, getz p in
-  let is_rz_x = fmul_eq_vartime r_fe z x in
-  let res =
+  let h2 = ST.get () in
+  fnormalize tmp_x x;
+  let h3 = ST.get () in
+  BL.normalize5_lemma (1,1,1,1,2) (as_felem5 h2 x);
+  //assert (inv_fully_reduced h3 tmp_x);
+  //assert (inv_lazy_reduced2 h3 z);
+
+  let is_rz_x = fmul_eq_vartime r_fe z tmp_x in
+  //assert (is_rz_x == (S.fmul (as_nat h3 r_fe) (feval h3 z) = as_nat h3 tmp_x));
+
+  let res : bool =
     if not is_rz_x then begin
      let is_r_lt_p_m_q = is_felem_lt_prime_minus_order_vartime r_fe in
      if is_r_lt_p_m_q then begin
-       make_u64_4 tmp (make_order_k256 ());
-       fadd tmp r tmp;
-       fmul_eq_vartime tmp z x end
+       assert (as_nat h1 r_fe < S.prime - S.q);
+       make_u52_5 tmp_q (make_order_k256 ());
+       let h4 = ST.get () in
+       BL.add5_lemma (1,1,1,1,1) (1,1,1,1,1) (as_felem5 h4 r_fe) (as_felem5 h4 tmp_q);
+       fadd tmp_q r_fe tmp_q;
+       fmul_eq_vartime tmp_q z tmp_x end
+       //assert (is_rqz_x == (S.fmul (feval h5 tmp) (feval h5 z) = as_nat h5 tmp_x));
      else false end
     else true in
 
-  KL.ecdsa_verify_avoid_finv (point_as_nat3_proj h0 p) (qas_nat h0 r);
   pop_frame ();
+  KL.ecdsa_verify_avoid_finv (point_eval h0 p) (qas_nat h0 r);
+  assert (res <==> (S.fmul (feval h0 x) (S.finv (feval h0 z)) % S.q = qas_nat h0 r));
+  let h5 = ST.get () in
+  assert (modifies0 h0 h5);
   res
 
 
@@ -137,12 +164,12 @@ val ecdsa_verify_qelem_aff (pk_x pk_y:felem) (z r s:qelem) : Stack bool
     live h pk_x /\ live h pk_y /\ live h z /\ live h r /\ live h s /\
     qas_nat h z < S.q /\ qas_nat h s < S.q /\
     0 < qas_nat h r /\ qas_nat h r < S.q /\
-    fe_lt_prime h pk_x /\ fe_lt_prime h pk_y)
+    inv_fully_reduced h pk_x /\ inv_fully_reduced h pk_y)
   (ensures  fun h0 b h1 -> modifies0 h0 h1 /\
    (let sinv = S.qinv (qas_nat h0 s) in
     let u1 = S.qmul (qas_nat h0 z) sinv in
     let u2 = S.qmul (qas_nat h0 r) sinv in
-    let p = (as_nat h0 pk_x, as_nat h0 pk_y, S.one) in
+    let p = (feval h0 pk_x, feval h0 pk_y, S.one) in
     let _X, _Y, _Z = S.point_mul_double_g u1 u2 p in
     b <==> (if S.is_proj_point_at_inf (_X, _Y, _Z) then false
       else S.fmul _X (S.finv _Z) % S.q = qas_nat h0 r)))
@@ -186,9 +213,13 @@ let ecdsa_verify_hashed_msg m public_key_x public_key_y r s =
   let is_s_valid = load_qelem_vartime s_q s in
   load_qelem_modq z m;
 
+  let h0 = ST.get () in
   let res =
     if not (is_xy_on_curve && is_r_valid && is_s_valid) then false
-    else ecdsa_verify_qelem_aff pk_x pk_y z r_q s_q in
+    else begin
+      Math.Lemmas.small_mod (as_nat h0 pk_x) S.prime;
+      Math.Lemmas.small_mod (as_nat h0 pk_y) S.prime;
+      ecdsa_verify_qelem_aff pk_x pk_y z r_q s_q end in
   pop_frame ();
   res
 #pop-options
